src/example/Client01.v
@@ -287,7 +287,7 @@ Section SPEC.
       { eauto. }
       { iFrame. }
       iIntros "DUTY CRD2". rred2r.
-      
+
       (* Appeal to the inductive hypothesis *)
       iInv "INV" as "CI" "CI_CLOSE".
       iEval (unfold client01Inv; simpl; red_tl_all; rewrite red_syn_until_tpromise; simpl) in "CI".
@@ -346,11 +346,11 @@ Section SPEC.
     Let init_ord := Ord.O.
     (* Let init_ord := layer 2 1. *)
     Let init_ths :=
-          (NatStructsLarge.NatMap.add
+          (NatStructs.NatMap.add
              tid1 tt
-             (NatStructsLarge.NatMap.add
+             (NatStructs.NatMap.add
                 tid2 tt
-                (NatStructsLarge.NatMap.empty unit))).
+                (NatStructs.NatMap.empty unit))).
 
     Let idx := 1.
 
@@ -429,16 +429,16 @@ Section SPEC.
       unfold WSim.initial_prop.
       iDestruct "INIT" as "(INIT0 & INIT1 & INIT2 & INIT3 & INIT4 & INIT5)".
       (* make thread_own, duty *)
-      assert (NatStructsLarge.NatMap.find tid1 init_ths = Some tt).
-      { unfold init_ths. apply NatStructsLarge.nm_find_add_eq. }
+      assert (NatStructs.NatMap.find tid1 init_ths = Some tt).
+      { unfold init_ths. apply NatStructs.nm_find_add_eq. }
       iPoseProof (natmap_prop_remove_find _ _ _ H with "INIT2") as "[DU1 INIT2]".
       iPoseProof (natmap_prop_remove_find _ _ _ H with "INIT3") as "[TH1 INIT3]".
       clear H.
-      assert (NatStructsLarge.NatMap.find tid2 (NatStructsLarge.NatMap.remove tid1 init_ths) = Some tt).
+      assert (NatStructs.NatMap.find tid2 (NatStructs.NatMap.remove tid1 init_ths) = Some tt).
       { unfold init_ths.
-        rewrite NatStructsLarge.NatMapP.F.remove_neq_o; ss.
-        rewrite NatStructsLarge.nm_find_add_neq; ss.
-        rewrite NatStructsLarge.nm_find_add_eq. ss.
+        rewrite NatStructs.NatMapP.F.remove_neq_o; ss.
+        rewrite NatStructs.nm_find_add_neq; ss.
+        rewrite NatStructs.nm_find_add_eq. ss.
       }
       iPoseProof (natmap_prop_remove_find _ _ _ H with "INIT2") as "[DU2 INIT2]".
       iPoseProof (natmap_prop_remove_find _ _ _ H with "INIT3") as "[TH2 INIT3]".
