src/example/Client05.v
@@ -35,14 +35,14 @@ Module Client05.
                           _ <- Spinlock.unlock L;;
                           Ret (inl d))
                     else Ret (inr tt)) d.
-    
+
     Definition thread2 :
       ktree (threadE ident state) unit unit
       :=
       fun _ =>
         _ <- OMod.call (R:=unit) "store" (D, (SCMem.val_nat 1));;
         Ret tt.
-    
+
     Definition omod : Mod.t :=
       Mod.mk
         tt
@@ -298,7 +298,7 @@ Section SPEC.
     iInv "INV" as "TI" "TI_CLOSE". iEval (simpl; unfold client05Inv; red_tl_all; simpl) in "TI".
     iDestruct "TI" as "[[PEND' PTD] | [#SHOT _]]"; cycle 1.
     { iExFalso. iApply (OneShots.pending_not_shot with "PEND SHOT"). }
-    
+
     iPoseProof (OneShots.pending_merge _ (1/2) (1/2) with "PEND PEND'") as "PEND". rewrite Qp.half_half.
     iMod (OneShots.pending_shot with "PEND") as "#SHOT".
     iMod (duty_fulfill with "[DUTY]") as "DUTY".
@@ -309,7 +309,7 @@ Section SPEC.
     iIntros (rv) "PTD". rred2r. iApply wpsim_tauR. rred2r. lred2r.
     iMod ("TI_CLOSE" with "[PTD]") as "_".
     { unfold client05Inv; simpl; red_tl_all; simpl. iRight; auto. }
-    
+
     iApply wpsim_ret. auto. iModIntro. unfold term_cond; iFrame; iPureIntro; reflexivity.
   Qed.
 
@@ -319,11 +319,11 @@ Section SPEC.
     Variable tid1 tid2 : thread_id.
     Let init_ord := Ord.O.
     Let init_ths :=
-          (NatStructsLarge.NatMap.add
+          (NatStructs.NatMap.add
              tid1 tt
-             (NatStructsLarge.NatMap.add
+             (NatStructs.NatMap.add
                 tid2 tt
-                (NatStructsLarge.NatMap.empty unit))).
+                (NatStructs.NatMap.empty unit))).
 
     Let idx := 1.
 
@@ -374,16 +374,16 @@ Section SPEC.
       unfold WSim.initial_prop.
       iDestruct "INIT" as "(INIT0 & INIT1 & INIT2 & INIT3 & INIT4 & INIT5)".
       (* make thread_own, duty *)
-      assert (NatStructsLarge.NatMap.find tid1 init_ths = Some tt).
-      { unfold init_ths. apply NatStructsLarge.nm_find_add_eq. }
+      assert (NatStructs.NatMap.find tid1 init_ths = Some tt).
+      { unfold init_ths. apply NatStructs.nm_find_add_eq. }
       iPoseProof (natmap_prop_remove_find _ _ _ H with "INIT2") as "[DU1 INIT2]".
       iPoseProof (natmap_prop_remove_find _ _ _ H with "INIT3") as "[TH1 INIT3]".
       clear H.
-      assert (NatStructsLarge.NatMap.find tid2 (NatStructsLarge.NatMap.remove tid1 init_ths) = Some tt).
+      assert (NatStructs.NatMap.find tid2 (NatStructs.NatMap.remove tid1 init_ths) = Some tt).
       { unfold init_ths.
-        rewrite NatStructsLarge.NatMapP.F.remove_neq_o; ss.
-        rewrite NatStructsLarge.nm_find_add_neq; ss.
-        rewrite NatStructsLarge.nm_find_add_eq. ss.
+        rewrite NatStructs.NatMapP.F.remove_neq_o; ss.
+        rewrite NatStructs.nm_find_add_neq; ss.
+        rewrite NatStructs.nm_find_add_eq. ss.
       }
       iPoseProof (natmap_prop_remove_find _ _ _ H with "INIT2") as "[DU2 INIT2]".
       iPoseProof (natmap_prop_remove_find _ _ _ H with "INIT3") as "[TH2 INIT3]".
