src/example/ClientSpinlock2.v
@@ -105,7 +105,7 @@ Section SIM.
   Context {TLRAS : TLRAs STT Γ Σ}.
 
   Context {HasMEMRA: @GRA.inG memRA Γ}.
-  
+
   Context {HasOneShotsNat : @GRA.inG (OneShots.t unit) Γ}.
   Context {HasAuthExcls : @GRA.inG (AuthExcls.t (nat * nat)) Γ}.
 
@@ -225,7 +225,7 @@ Section SIM.
     iDestruct "POST" as (γκu') "POST". iEval (red_tl; simpl) in "POST".
     iDestruct "POST" as (κu') "POST". iEval (red_tl_all; simpl) in "POST".
     iDestruct "POST" as "(LW & _ & DUTY & PC)". rred2r.
-    
+
     iMod (pcs_decr _ _ 1 2 3 with "PCS") as "[PCS' PCS]". auto.
     iApply (wpsim_yieldR with "[DUTY PCS' PC]"). auto.
     { iFrame. iApply (pcs_cons_fold with "[PCS' PC]"). iFrame. }
@@ -235,12 +235,12 @@ Section SIM.
     iEval (unfold clientSpinlock2_inv; simpl; red_tl_all; simpl) in "CI".
     iDestruct "CI" as "[(PTD & #OBLw & #PRMw & LIVE' & #OBLu & #DPRMu & PO2 & LIVE2) | (_ & #SHOT & _)]"; cycle 1.
     { iExFalso. iApply (OneShots.pending_not_shot with "LIVE SHOT"). }
-    
+
     iApply (SCMem_store_fun_spec with "[PTD]"). auto.
     { pose proof md_N_ClientSpinlock2_state_tgt. set_solver. }
     { iFrame. auto. }
     iIntros (rv) "PTD". rred2r. iApply wpsim_tauR. rred2r.
-    
+
     iPoseProof (pass_lock with "[LW DUTY PCs PO2 LIVE2]") as "PASS".
     2:{ red_tl_all. repeat iSplit; auto. iFrame. simpl. repeat iSplit; auto. }
     { instantiate (1 := ⊤ ∖ ↑N_ClientSpinlock2). pose proof md_N_ClientSpinlock2_Spinlock. set_solver. }
@@ -255,7 +255,7 @@ Section SIM.
 
     iMod ("CI_CLOSE" with "[PTD LW]") as "_".
     { iEval (unfold clientSpinlock2_inv; simpl). red_tl_all. iRight. iFrame. done. }
-    
+
     iApply (wpsim_sync2 with "[DUTY]"). auto. auto. iFrame.
     iIntros "DUTY _ _". simpl. rred2r. iApply wpsim_tauR. rred2r. lred2r.
 
@@ -370,7 +370,7 @@ Section SIM.
         iApply (wpsim_yieldR2 with "[DUTY PCS]"). auto. 2: { iFrame. done. } lia.
         iIntros "DUTY _ PCS". simpl. rred2r.
         iApply wpsim_tauR. rred2r.
-        
+
         iMod (pcs_decr _ _ 1 with "PCS") as "[PCS' PCS]". left.
         iApply (Spinlock_unlock_spec with "[DUTY LW PCS']").
         { pose proof md_Spinlock_state_tgt. set_solver. }
@@ -420,7 +420,7 @@ Section SIM.
       iApply (wpsim_yieldR2 with "[DUTY PCS]"). auto. 2: { iFrame. done. } lia.
       iIntros "DUTY _ PCS". simpl. rred2r.
       iApply wpsim_tauR. rred2r.
-      
+
       iMod (pcs_decr _ _ 1 with "PCS") as "[PCS' PCS]". left.
       iApply (Spinlock_unlock_spec with "[DUTY LW PCS']").
       { pose proof md_Spinlock_state_tgt. set_solver. }
@@ -438,11 +438,11 @@ Section SIM.
   Variable tid1 tid2 : thread_id.
   Let init_ord := Ord.O.
   Let init_ths :=
-        (NatStructsLarge.NatMap.add
+        (NatStructs.NatMap.add
            tid1 tt
-           (NatStructsLarge.NatMap.add
+           (NatStructs.NatMap.add
               tid2 tt
-              (NatStructsLarge.NatMap.empty unit))).
+              (NatStructs.NatMap.empty unit))).
 
   Let idx := 1.
 
@@ -483,16 +483,16 @@ Section SIM.
     unfold WSim.initial_prop.
     iDestruct "INIT" as "(INIT0 & INIT1 & INIT2 & INIT3 & INIT4 & INIT5)".
     (* make thread_own, duty *)
-    assert (NatStructsLarge.NatMap.find tid1 init_ths = Some tt).
-    { unfold init_ths. apply NatStructsLarge.nm_find_add_eq. }
+    assert (NatStructs.NatMap.find tid1 init_ths = Some tt).
+    { unfold init_ths. apply NatStructs.nm_find_add_eq. }
     iPoseProof (natmap_prop_remove_find _ _ _ H with "INIT2") as "[DU1 INIT2]".
     iPoseProof (natmap_prop_remove_find _ _ _ H with "INIT3") as "[TH1 INIT3]".
     clear H.
-    assert (NatStructsLarge.NatMap.find tid2 (NatStructsLarge.NatMap.remove tid1 init_ths) = Some tt).
+    assert (NatStructs.NatMap.find tid2 (NatStructs.NatMap.remove tid1 init_ths) = Some tt).
     { unfold init_ths.
-      rewrite NatStructsLarge.NatMapP.F.remove_neq_o; ss.
-      rewrite NatStructsLarge.nm_find_add_neq; ss.
-      rewrite NatStructsLarge.nm_find_add_eq. ss.
+      rewrite NatStructs.NatMapP.F.remove_neq_o; ss.
+      rewrite NatStructs.nm_find_add_neq; ss.
+      rewrite NatStructs.nm_find_add_eq. ss.
     }
     iPoseProof (natmap_prop_remove_find _ _ _ H with "INIT2") as "[DU2 INIT2]".
     iPoseProof (natmap_prop_remove_find _ _ _ H with "INIT3") as "[TH2 INIT3]".
