src/example/OneShotsRA.v
@@ -23,7 +23,7 @@ Module OneShots.
       shot k a -∗ □ shot k a.
     Proof.
       iIntros "H". iPoseProof (own_persistent with "H") as "H".
-      rewrite FiniteMap.singleton_core. auto.
+      rewrite FiniteMap.singleton_core_total. auto.
     Qed.
 
     Global Program Instance Persistent_shot k a : Persistent (shot k a).
