src/ra/FairnessRA.v
@@ -2,7 +2,7 @@ From iris.algebra Require Import cmra updates.
 From sflib Require Import sflib.
 From Fairness Require Import WFLibLarge Mod Optics.
 From Fairness Require Import PCM IProp IPM IPropAux.
-From Fairness Require Import NatMapRALarge MonotoneRA.
+From Fairness Require Import NatMapRA MonotoneRA.
 Require Import Coq.Classes.RelationClasses.
 Require Import Coq.Logic.PropExtensionality.
 From Fairness Require Import Axioms.
